Début du système de déduction naturelle pour HOL.

src/HOL/Theorie.v
@@ -1,32 +1,71 @@
-From CRM Require Import Base Typing unscoped.
+From CRM Require Import Base Typing fintype.
+Import CombineNotations SubstNotations.
 
-From Stdlib Require Import PeanoNat List.
+From Stdlib Require Import PeanoNat List Datatypes.
+Import ListNotations.
 
 Reserved Notation "Γ | Ξ ⊢ φ" (at level 85).
 
-Definition eq_tm (t : tm) (u : tm) : tm :=
-  ∀ₛ ((⟦ 0 ⟧ₛ @ₛ ren_tm shift t) ⇒ₛ (⟦ 0 ⟧ₛ @ₛ ren_tm shift t)).
-
-Definition ex_tm (φ : tm) : tm :=
-  ∀ₛ (∀ₛ (ren_tm shift φ ⇒ₛ ⟦ 1 ⟧ₛ) ⇒ₛ ⟦ 0 ⟧ₛ).
-
-Lemma typ_eq_tm : forall (Γ : HOL_ctx) (s : st) (t : tm) (u : tm),
-    Γ ⊢ t ~: s -> Γ ⊢ u ~: s -> Γ ⊢ eq_tm t u ~: ℙₛ.
+Definition shift11 {n : nat} (g : fin (S n)) : fin (S (S n)).
 Proof.
-  intros. apply (@HOL_typ_forall _ (s →ₛ ℙₛ)).
-  constructor. apply (@HOL_typ_app _ _ s).
-  constructor. constructor.
-  admit.
-  apply (@HOL_typ_app _ _ s). constructor. constructor.
-  admit.
-Admitted.
+  destruct g.
+  - apply Some. apply Some. apply f.
+  - apply None.
+Defined.
 
-Lemma typ_ex_tm : forall (Γ : HOL_ctx) (s : st) (φ : tm),
-    s :: Γ ⊢ φ ~: ℙₛ -> Γ ⊢ ex_tm φ ~: ℙₛ.
+Lemma typ_shift : forall (n : nat) (Γ : HOL_ctx n)
+                         (s s' s0: st) (t : tm (S n)),
+    s .: Γ ⊢⟨ S n ⟩ t ~: s0 ->
+    s .: (s' .: Γ) ⊢⟨ S (S n) ⟩ ren_tm shift11 t ~: s0.
 Proof.
-  intros. apply (@HOL_typ_forall _ ℙₛ).
-  constructor. apply (@HOL_typ_forall _ s). constructor.
-  admit.
-  constructor. constructor. constructor.
+  intros. apply (typ_ren (S (S n)) (S n) shift11 (s .: (s' .: Γ)) (s .: Γ)).
+  intro. unfold ">>"; simpl. case f; reflexivity.
+  apply H.
+Qed.
+
+Definition ex_tm {n : nat} (φ : tm (S n)) : tm n.
+Proof.
+  apply forall_tm. apply imp_tm.
+  apply forall_tm. apply imp_tm.
+  exact (ren_tm shift11 φ). apply var_tm. apply Some. apply None.
+  apply var_tm. apply None.
+Defined.
+
+Notation "∃ₛ" := (ex_tm).
+
+Lemma typ_ex_tm : forall (n : nat) (Γ : HOL_ctx n) (s : st) (φ : tm (S n)),
+    s .: Γ ⊢⟨ S n ⟩ φ ~: ℙₛ -> Γ ⊢⟨ n ⟩ ex_tm φ ~: ℙₛ.
+Proof.
+  intros. apply (typ_forall ℙₛ).
+  constructor. apply (typ_forall s). constructor.
+  apply typ_shift. apply H.
   constructor. constructor.
-Admitted.
+Qed.
+
+Definition eq_tm {n : nat} (t : tm n) (u : tm n) : tm n.
+Proof.
+  apply forall_tm. apply imp_tm.
+  apply app_tm. apply var_tm; apply None.
+  exact (ren_tm shift t).
+  apply app_tm. apply var_tm; apply None.
+  exact (ren_tm shift u).
+Defined.
+
+Notation "t =ₛ u" := (eq_tm t u) (at level 86).
+
+Lemma typ_eq_tm : forall (n : nat) (Γ : HOL_ctx n) (s : st)
+                         (t : tm n) (u : tm n),
+    Γ ⊢⟨ n ⟩ t ~: s -> Γ ⊢⟨ n ⟩ u ~: s -> Γ ⊢⟨ n ⟩ t =ₛ u ~: ℙₛ.
+Proof.
+  intros. apply (typ_forall (s →ₛ ℙₛ)).
+  constructor. apply (typ_app s).
+  constructor. apply typ_weaken. apply H.
+  apply (typ_app s). constructor. apply typ_weaken. apply H0.
+Qed.
+
+Definition proof_ctx (n : nat) (Γ : fin n -> st) := list (tm n).
+
+Inductive wt_ctx {n : nat} {Γ : fin n -> st} : proof_ctx n -> Prop :=
+| wt_nil : wt_ctx nil
+| wt_cons : forall {Ξ : proof_ctx n} {φ : tm n},
+    wt_ctx Ξ -> (Γ ⊢⟨ n ⟩ φ ~: ℙₛ) -> wt_ctx (φ :: Ξ).
